---
title: "hw2"
format: pdf
editor: visual
---

# Problem 1

![](images/WeChat065c203038c7e29ee155cea4a3a9dfe8.png)

**Answer:**

$SSR=\sum(\hat{Y}-\bar{Y})^2$

Since $(\bar{X},\bar{Y})$ must be on the estimated regression line.

$SSR=\sum(\hat{\beta_0}+\hat{\beta_1}X_i-\hat{\beta_0}-\hat{\beta_1}\bar{X})$

$SSR=\hat{\beta_1^2}\sum(X_i-\bar{X})^2$

$F=\frac{MSR}{MSE}=\frac{\frac{SSR}{1}}{\frac{SSE}{n-2}}=\frac{\hat{\beta_1^2}\sum(X_i-\bar{X})^2}{MSE}$

$SE(\hat{\beta_1})=\frac{\sqrt{MSE}}{\sqrt{\sum(X_i-\bar{X})^2}}$

Hence:

$F=\frac{\hat{\beta_1^2}}{SE(\hat{\beta_1})^2}=(\frac{\hat{\beta_1}}{SE(\hat{\beta_1})})^2=t^2$

# Problem 2

![](images/WeChatcbdaa452ae5d71d7c3dbd5b3de1dbe83.png)

Note:

$\hat{\beta_1}=\frac{\sum(X_i-\bar{X})(Y_i-\bar{Y})}{\sum(X_i-\bar{X})^2}$

$\hat{\beta_0}=\bar{Y}-\hat{\beta_1}\bar{X}$

$\hat{\sigma}^2=\frac{1}{n-2}\sum(Y_i-\bar{Y_i})^2$

$R^2=\frac{SSR}{SSTO}=\frac{\sum(\hat{Y_i}-\bar{Y})^2}{\sum(Y_i-\bar{Y})^2}$

**(a) Answer:**

Given $x_i$ is replaced be $cx_i$,

$\hat{\beta_1^*}=\frac{\sum(cX_i-c\bar{X})(Y_i-\bar{Y})}{\sum(cX_i-c\bar{X})^2}=\frac{c\sum(X_i-\bar{X})(Y_i-\bar{Y})}{c^2\sum(X_i-\bar{X})^2}=\frac{\sum(X_i-\bar{X})(Y_i-\bar{Y})}{c\sum(X_i-\bar{X})^2}=\frac{1}{c}\hat{\beta_1}$

$\hat{\beta_0^*}=\bar{Y}-\hat{\beta_1^*}(c\bar{X})=\hat{\beta_0}$

$\hat{\sigma^*}^2=\frac{1}{n-2}\sum(Y_i-\bar{Y_i})^2=\hat{\sigma}^2$

$R^{*2}=\frac{\sum(\hat{Y_i^*}-\bar{Y})^2}{\sum(Y_i-\bar{Y})^2}=\frac{\sum(\hat{\beta_0^*}+\hat{\beta_1^*}X_i-\bar{Y})^2}{\sum(Y_i-\bar{Y})^2}=\frac{\sum(\hat{\beta_0}+\frac{1}{c}\hat{\beta_1}X_i-\bar{Y})^2}{\sum(Y_i-\bar{Y})^2}$

**(b) Answer:**

Given $x_i$ is replaced be $x_i+d$,

$\hat{\beta_1^*}=\frac{\sum((X_i+d)-(\bar{X}+d))(Y_i-\bar{Y})}{\sum((X_i+d)-(\bar{X}+d))^2}=\frac{\sum(X_i-\bar{X})(Y_i-\bar{Y})}{\sum(X_i-\bar{X})^2}=\hat{\beta_1}$

$\hat{\beta_0^*}=\bar{Y}-\hat{\beta_1^*}(\bar{X}+d)=\bar{Y}-\hat{\beta_1}(\bar{X}+d)=\bar{Y}-\hat{\beta_1}\bar{X}-\hat{\beta_1}d$

$\hat{\sigma^*}^2=\frac{1}{n-2}\sum(Y_i-\bar{Y_i})^2=\hat{\sigma}^2$

$R^{*2}=\frac{\sum(\hat{Y_i^*}-\bar{Y})^2}{\sum(Y_i-\bar{Y})^2}=\frac{\sum(\hat{\beta_0^*}+\hat{\beta_1^*}X_i-\bar{Y})^2}{\sum(Y_i-\bar{Y})^2}=\frac{\sum(\bar{Y}-\hat{\beta_1}\bar{X}-\hat{\beta_1}d+\hat{\beta_1}(X_i+d)-\bar{Y})^2}{\sum(Y_i-\bar{Y})^2}=\frac{\sum(-\hat{\beta_1}\bar{X}+\hat{\beta_1}X_i)^2}{\sum(Y_i-\bar{Y})^2}=\frac{\hat{\beta_1}^2\sum(X_i-\bar{X})^2}{\sum(Y_i-\bar{Y})^2}$

**(c) Answer:**

Given $y_i$ is replaced be $ky_i$,

$\hat{\beta_1^*}=\frac{\sum(X_i-\bar{X})(kY_i-k\bar{Y})}{\sum(X_i-\bar{X})^2}=\frac{k\sum(X_i-\bar{X})(Y_i-\bar{Y})}{\sum(X_i-\bar{X})^2}=k\hat{\beta_1}$

$\hat{\beta_0^*}=k\bar{Y}-\hat{\beta_1^*}\bar{X}=k\bar{Y}-k\hat{\beta_1}\bar{X}=k(\bar{Y}-\hat{\beta_1}\bar{X})=k\hat{\beta_0}$

$\hat{\sigma^*}^2=\frac{1}{n-2}\sum(kY_i-k\bar{Y_i})^2=\frac{k^2}{n-2}\sum(Y_i-\bar{Y_i})^2=k^2\hat{\sigma}^2$

$R^{*2}=\frac{\sum(\hat{Y_i^*}-k\bar{Y})^2}{\sum(kY_i-k\bar{Y})^2}=\frac{\sum(\hat{\beta_0^*}+\hat{\beta_1^*}X_i-k\bar{Y})^2}{\sum(kY_i-k\bar{Y})^2}=\frac{\sum(k\hat{\beta_0}+k\hat{\beta_1}X_i-k\bar{Y})^2}{\sum(kY_i-k\bar{Y})^2}=\frac{k^2\sum(\hat{\beta_0}+\hat{\beta_1}X_i-\bar{Y})^2}{k^2\sum(Y_i-\bar{Y})^2}=R^2$

**(d) Answer:**

Given $y_i$ is replaced be $y_i+d$,

$\hat{\beta_1^*}=\frac{\sum(X_i-\bar{X})(Y_i+d-\bar{Y}-d)}{\sum(X_i-\bar{X})^2}=\frac{\sum(X_i-\bar{X})(Y_i-\bar{Y})}{\sum(X_i-\bar{X})^2}=\hat{\beta_1}$

$\hat{\beta_0^*}=\bar{Y}+d-\hat{\beta_1^*}\bar{X}=\bar{Y}+d-\hat{\beta_1}\bar{X}=\hat{\beta_0}+d$

$\hat{\sigma^*}^2=\frac{1}{n-2}\sum(Y_i+d-\bar{Y_i}-d)^2=\frac{1}{n-2}\sum(Y_i-\bar{Y_i})^2=\hat{\sigma}^2$

$R^{*2}=\frac{\sum(\hat{Y_i^*}-\bar{Y}-d)^2}{\sum(Y_i+d-\bar{Y_i}-d)^2}=\frac{\sum(\hat{\beta_0^*}+\hat{\beta_1^*}X_i-\bar{Y}-d)^2}{\sum(Y_i-\bar{Y})^2}=\frac{\sum(\hat{\beta_0}+d+\hat{\beta_1}X_i-\bar{Y}-d)^2}{\sum(Y_i-\bar{Y})^2}=\frac{\sum(\hat{Y_i}-\bar{Y})^2}{\sum(Y_i-\bar{Y})^2}=R^2$

**(e) Answer:**

# Problem 3

![](images/WeChat3952ce67e4ef94d72d2391a272c0f795.png)

# Problem 4

![](images/WeChatb2e8b640c9aea08a816ff2005aacd55c.png)

**(a) Answer:**

$\frac{\sum(X_i-\bar{X})(Y_i-\bar{Y})}{\sum(X_i-\bar{X})^2}=\frac{\sum(X_iY_i-X_i\bar{Y}-\bar{X}Y_i+\bar{X}\bar{Y})}{\sum(X_i-\bar{X})^2}$

$\frac{\sum(X_i-\bar{X})(Y_i-\bar{Y})}{\sum(X_i-\bar{X})^2}=\frac{\sum(X_iY_i-X_i\bar{Y}-\bar{X}Y_i)+n\frac{\sum{X_i}}{n}\bar{Y}}{\sum(X_i-\bar{X})^2}$

$\frac{\sum(X_i-\bar{X})(Y_i-\bar{Y})}{\sum(X_i-\bar{X})^2}=\frac{\sum(X_iY_i-X_i\bar{Y}-\bar{X}Y_i+X_i\bar{Y})}{\sum(X_i-\bar{X})^2}$

$\frac{\sum(X_i-\bar{X})(Y_i-\bar{Y})}{\sum(X_i-\bar{X})^2}=\frac{\sum(X_iY_i-\bar{X}Y_i)}{\sum(X_i-\bar{X})^2}$

$\frac{\sum(X_i-\bar{X})(Y_i-\bar{Y})}{\sum(X_i-\bar{X})^2}=\frac{\sum(X_i-\bar{X})Y_i}{\sum(X_i-\bar{X})^2}$

**(b) Answer:**

$Cov(\bar{Y},\hat{\beta_1})=E[\bar{Y}\hat{\beta_1}]-E[\bar{Y}]E[\hat{\beta_1}]=\bar{Y}E[\hat{\beta_1}]-\bar{Y}E[\hat{\beta_1}]=0$
