---
title: "hw6"
author: "Hanbei Xiong"
format: html
editor: visual
---

# Question 1

![](images/WeChatd86e31862e0f89c52c04f8db62e1414c.png)

**(a) Answer:**

```{=tex}
\begin{align*}
\hat{\beta}_{(-i)}&=(X_{(-i)}'X_{(-i)})^{-1}X_{(-i)}'Y_{(-i)}\\
&=[(X'X)^{-1}+\frac{(X'X)^{-1}x_ix_i'(X'X)^{-1}}{1-h_i}](X'Y-x_iY_i)\\
&=(X'X)^{-1}X'Y-(X'X)^{-1}x_iY_i+(\frac{(X'X)^{-1}x_ix_i'(X'X)^{-1}}{1-h_i})X'Y-(\frac{(X'X)^{-1}x_ix_i'(X'X)^{-1}}{1-h_i})x_iY_i\\
&=\hat{\beta}-\frac{(X'X)^{-1}x_iY_i}{1-h_i}+(\frac{(X'X)^{-1}x_ix_i'(X'X)^{-1}}{1-h_i})x_iY_i\\
&+(\frac{(X'X)^{-1}x_ix_i'(X'X)^{-1}}{1-h_i})X'Y-(\frac{(X'X)^{-1}x_ix_i'(X'X)^{-1}}{1-h_i})x_iY_i\\
&=\hat{\beta}-\frac{(X'X)^{-1}x_iY_i}{1-h_i}+(\frac{(X'X)^{-1}x_ix_i'(X'X)^{-1}}{1-h_i})X'Y\\
&=\hat{\beta}-\frac{(X'X)^{-1}x_iY_i}{1-h_i}+(\frac{(X'X)^{-1}x_ix_i'(X'X)^{-1}}{1-h_i})X'X\beta\\
&=\hat{\beta}-\frac{(X'X)^{-1}x_iY_i}{1-h_i}+\frac{(X'X)^{-1}x_ix_i'\beta}{1-h_i}\\
&=\hat{\beta}-\frac{(X'X)^{-1}x_i(Y_i-x_i'\beta)}{1-h_i}\\
&=\hat{\beta}-\frac{(X'X)^{-1}x_ie_i}{1-h_i}
\end{align*}
```

**(b) Answer:**

\begin{align*}
y_i-x'_{i}\hat{\beta}_{(-i)}&=y_i-x'_i(\hat{\beta}-\frac{(X'X)^{-1}x_ie_i}{1-h_i})\\
&=y_i-x'_i\hat{\beta}+\frac{x'_i(X'X)^{-1}x_ie_i}{1-h_i}\\
&=\frac{(x'_i\hat{\beta}+e_i)(1-h_i)}{1-h_i}-\frac{x'_i\hat{\beta}(1-h_i)}{1-h_i}+\frac{h_ie_i}{1-h_i}\\
&=\frac{e_i(1-h_i)}{1-h_i}+\frac{h_ie_i}{1-h_i}\\
&=\frac{e_i(1-h_i+h_i)}{1-h_i}\\
&=\frac{e_i}{1-h_i}
\end{align*}

# Question 2

![](images/WeChatd1bf81cdec0eb521ce0ff93608b25575.png)

# Question 3

![](images/WeChat6a6d80ee6a3962848a263b5604785992.png)
